cfrontend/BeePL_auxlemmas.v
@@ -1,0 +1,188 @@
+Require Import String ZArith Coq.FSets.FMapAVL Coq.Structures.OrderedTypeEx.
+Require Import Coq.FSets.FSetProperties Coq.FSets.FMapFacts FMaps FSetAVL Nat PeanoNat.
+Require Import Coq.Arith.EqNat Coq.ZArith.Int Integers AST Maps Linking Ctypes.
+Require Import BeePL_aux BeePL_mem BeeTypes BeePL Csyntax Clight Globalenvs BeePL_Csyntax SimplExpr.
+Require Import compcert.common.Errors.
+
+From mathcomp Require Import all_ssreflect. 
+
+Lemma extract_type_notbool : forall v t v',
+sem_unary_operation Notbool v t = Some v' -> 
+t = Ptype Tbool.
+Proof.
+move=> v t v' /= hs. rewrite /sem_notbool /= in hs.
+move: hs. case: v=> //=.
++ case: t=> //= p. by case: p=> //=.
++ case: t=> //= p. by case: p=> //=.
++ case: t=> //= p. case: p=> //=.
+case: t=> //= i b. case: b=> //= p. case: p=> //=.
+Qed.
+
+Lemma extract_type_notint : forall v t v',
+sem_unary_operation Notint v t = Some v' -> 
+exists sz s, t = Ptype (Tint sz s).
+Proof.
+move=> v t v' /= hs. rewrite /sem_notint in hs.
+move: hs. case: v=> //=.
++ case: t=> //= p. by case: p=> //=.
++ case: t=> //= p i. case: p=> //= sz s [] hv; subst. 
+  by exists sz, s.
++ case: t=> //= p. by case: p=> //=.
+case: t=> //= i b. case: b=> //= p.
+by case: p=> //=.
+Qed.
+
+Lemma extract_type_neg : forall v t v',
+sem_unary_operation Neg v t = Some v' -> 
+exists sz s, t = Ptype (Tint sz s).
+Proof.
+move=> v t v' /= hs. rewrite /sem_notint in hs.
+move: hs. case: v=> //=.
++ case: t=> //= p. by case: p=> //=.
++ case: t=> //= p i. case: p=> //= sz s [] hv; subst. 
+  by exists sz, s.
++ case: t=> //= p. by case: p=> //=.
+case: t=> //= i b. case: b=> //= p.
+by case: p=> //=.
+Qed.
+ 
+Lemma extract_type_plus1 : forall v1 v2 t1 t2 v,
+sem_binary_operation Plus v1 v2 t1 t2 = Some v -> 
+exists sz s, t1 = Ptype (Tint sz s). 
+Proof.
+move=> v1 v2 t1 t2 v. rewrite /sem_binary_operation /sem_plus.
+case: v1=> //=.
++ case: v2=> //=. case: t1=> //= p. case: p=> //=.
+  case: t2=> //= p. by case: p=> //=.
++ case: v2=> //=. case: t1=> //= p i i'. case: p=> //= sz s.
+  case: t2=> //= p. case: p=> //= sz' s' [] hv; subst. by exists sz, s.
++ case: v2=> //=. case: t1=> //= p. case: p=> //=. case: t2=> //= p.
+  by case: p=> //=.
+case: v2=> //=. case: t1=> //= i b. case: b=> //= p.
+case: p=> //= sz s. case: t2=> //= b b'. case: b'=> //= p. by case: p.
+Qed.
+
+Lemma extract_type_plus2 : forall v1 v2 t1 t2 v,
+sem_binary_operation Plus v1 v2 t1 t2 = Some v -> 
+exists sz s, t2 = Ptype (Tint sz s). 
+Proof.
+move=> v1 v2 t1 t2 v. rewrite /sem_binary_operation /sem_plus.
+case: v1=> //=.
++ case: v2=> //=. case: t1=> //= p. case: p=> //=.
+  case: t2=> //= p. by case: p=> //=.
++ case: v2=> //=. case: t1=> //= p i i'. case: p=> //= sz s.
+  case: t2=> //= p. case: p=> //= sz' s' [] hv; subst. by exists sz', s'.
++ case: v2=> //=. case: t1=> //= p. case: p=> //=. case: t2=> //= p.
+  by case: p=> //=.
+case: v2=> //=. case: t1=> //= i b. case: b=> //= p.
+case: p=> //= sz s. case: t2=> //= b b'. case: b'=> //= p. by case: p.
+Qed.
+
+Lemma extract_type_minus1 : forall v1 v2 t1 t2 v,
+sem_binary_operation Minus v1 v2 t1 t2 = Some v -> 
+exists sz s, t1 = Ptype (Tint sz s). 
+Proof.
+move=> v1 v2 t1 t2 v. rewrite /sem_binary_operation /sem_minus.
+case: v1=> //=.
++ case: v2=> //=. case: t1=> //= p. case: p=> //=.
+  case: t2=> //= p. by case: p=> //=.
++ case: v2=> //=. case: t1=> //= p i i'. case: p=> //= sz s.
+  case: t2=> //= p. case: p=> //= sz' s' [] hv; subst. by exists sz, s.
++ case: v2=> //=. case: t1=> //= p. case: p=> //=. case: t2=> //= p.
+  by case: p=> //=.
+case: v2=> //=. case: t1=> //= i b. case: b=> //= p.
+case: p=> //= sz s. case: t2=> //= b b'. case: b'=> //= p. by case: p.
+Qed.
+
+Lemma extract_type_sub2 : forall v1 v2 t1 t2 v,
+sem_binary_operation Minus v1 v2 t1 t2 = Some v -> 
+exists sz s, t2 = Ptype (Tint sz s). 
+Proof.
+move=> v1 v2 t1 t2 v. rewrite /sem_binary_operation /sem_plus.
+case: v1=> //=.
++ case: v2=> //=. case: t1=> //= p. case: p=> //=.
+  case: t2=> //= p. by case: p=> //=.
++ case: v2=> //=. case: t1=> //= p i i'. case: p=> //= sz s.
+  case: t2=> //= p. case: p=> //= sz' s' [] hv; subst. by exists sz', s'.
++ case: v2=> //=. case: t1=> //= p. case: p=> //=. case: t2=> //= p.
+  by case: p=> //=.
+case: v2=> //=. case: t1=> //= i b. case: b=> //= p.
+case: p=> //= sz s. case: t2=> //= b b'. case: b'=> //= p. by case: p.
+Qed.
+
+Lemma extract_type_mult1 : forall v1 v2 t1 t2 v,
+sem_binary_operation Mult v1 v2 t1 t2 = Some v -> 
+exists sz s, t1 = Ptype (Tint sz s). 
+Proof.
+move=> v1 v2 t1 t2 v. rewrite /sem_binary_operation /sem_plus.
+case: v1=> //=.
++ case: v2=> //=. case: t1=> //= p. case: p=> //=.
+  case: t2=> //= p. by case: p=> //=.
++ case: v2=> //=. case: t1=> //= p i i'. case: p=> //= sz s.
+  case: t2=> //= p. case: p=> //= sz' s' [] hv; subst. by exists sz, s.
++ case: v2=> //=. case: t1=> //= p. case: p=> //=. case: t2=> //= p.
+  by case: p=> //=.
+case: v2=> //=. case: t1=> //= i b. case: b=> //= p.
+case: p=> //= sz s. case: t2=> //= b b'. case: b'=> //= p. by case: p.
+Qed.
+
+Lemma extract_type_mult2 : forall v1 v2 t1 t2 v,
+sem_binary_operation Mult v1 v2 t1 t2 = Some v -> 
+exists sz s, t2 = Ptype (Tint sz s). 
+Proof.
+move=> v1 v2 t1 t2 v. rewrite /sem_binary_operation /sem_plus.
+case: v1=> //=.
++ case: v2=> //=. case: t1=> //= p. case: p=> //=.
+  case: t2=> //= p. by case: p=> //=.
++ case: v2=> //=. case: t1=> //= p i i'. case: p=> //= sz s.
+  case: t2=> //= p. case: p=> //= sz' s' [] hv; subst. by exists sz', s'.
++ case: v2=> //=. case: t1=> //= p. case: p=> //=. case: t2=> //= p.
+  by case: p=> //=.
+case: v2=> //=. case: t1=> //= i b. case: b=> //= p.
+case: p=> //= sz s. case: t2=> //= b b'. case: b'=> //= p. by case: p.
+Qed.
+
+Lemma extract_type_div1 : forall v1 v2 t1 t2 v,
+sem_binary_operation Div v1 v2 t1 t2 = Some v -> 
+exists sz s, t1 = Ptype (Tint sz s). 
+Proof.
+move=> v1 v2 t1 t2 v. rewrite /sem_binary_operation /sem_div.
+case: v1=> //=.
++ case: v2=> //=. case: t1=> //= p. case: p=> //=.
+  case: t2=> //= p. by case: p=> //=.
++ case: v2=> //=. case: t1=> //= p i i'. case: p=> //= sz s.
+  case: t2=> //= p. case: p=> //= sz' s'. by exists sz, s.
++ case: v2=> //=. case: t1=> //= p. case: p=> //=. case: t2=> //= p.
+  by case: p=> //=.
+case: v2=> //=. case: t1=> //= i b. case: b=> //= p.
+case: p=> //= sz s. case: t2=> //= b b'. case: b'=> //= p. by case: p.
+Qed.
+
+Lemma extract_type_div2 : forall v1 v2 t1 t2 v,
+sem_binary_operation Div v1 v2 t1 t2 = Some v -> 
+exists sz s, t2 = Ptype (Tint sz s). 
+Proof.
+move=> v1 v2 t1 t2 v. rewrite /sem_binary_operation /sem_div.
+case: v1=> //=.
++ case: v2=> //=. case: t1=> //= p. case: p=> //=.
+  case: t2=> //= p. by case: p=> //=.
++ case: v2=> //=. case: t1=> //= p i i'. case: p=> //= sz s.
+  case: t2=> //= p. case: p=> //= sz' s'. by exists sz', s'.
++ case: v2=> //=. case: t1=> //= p. case: p=> //=. case: t2=> //= p.
+  by case: p=> //=.
+case: v2=> //=. case: t1=> //= i b. case: b=> //= p.
+case: p=> //= sz s. case: t2=> //= b b'. case: b'=> //= p. by case: p.
+Qed.
+
+Lemma int_gt_zero : forall i,
+Int.eq i Int.zero = false -> 
+(-1 < Int.intval i < Int.modulus)%Z ->
+(0 < Int.intval i)%Z.
+Proof.
+move=> [] i ir /= heq h. case: i ir heq h=> //=. 
+move=> p ir /= heq h. inversion h; subst. have hz := Zlt_neg_0 p.
+rewrite /Int.modulus /= /Int.wordsize /= /Wordsize_32.wordsize /two_power_nat /= in H0.
+by case: p ir heq h H hz H0=> //=.
+Qed.
+
+
